lit and seq verified

src/ASL/Theory.v
@@ -1,5 +1,5 @@
-From Coq   Require Import List ZArith.
-From ASL   Require Import Semantics.
+From Coq   Require Import List ZArith String.
+From ASL   Require Import AST Semantics.
 From ITree Require Import ITree ITreeFacts Events.MapDefaultFacts Events.StateFacts. 
 From Vellvm Require Import Semantics Syntax Theory.
 
@@ -7,7 +7,24 @@ Import SemNotations.
 Import ListNotations.
 Import ITreeNotations.
 
-Locate eutt.
+Definition dec_dec : forall s1 s2 : dec, {s1 = s2} + {s1 <> s2}.
+Proof.
+intros.
+destruct s1, s2.
+destruct (string_dec x x0) as [H_eq | H_neq];
+[ left; rewrite H_eq; reflexivity |
+  right; intros contra; inversion contra; apply H_neq; assumption].
+Qed.
+
+Fixpoint expr_dec (e1 e2 : expr) : {e1 = e2} + {e1 <> e2}.
+Proof.
+  decide equality. apply Int32.eq_dec.
+Defined.
+
+Fixpoint stmt_dec (s1 s2 : stmt) : {s1 = s2} + {s1 <> s2}.
+Proof.
+  decide equality; apply expr_dec || apply string_dec || auto.
+Defined.
 
 Lemma test4 {E} :
   forall (x:Semantics.env * unit),
@@ -85,6 +102,23 @@ Proof.
   rewrite unfold_interp. simpl.
   unfold MapDefault.interp_map. cbn.
   rewrite interp_state_ret.
+  reflexivity.
+Qed.
+
+
+
+Lemma interp_asl_bind {E} :
+  forall {R S} (t: itree (State +' E) R) (k: R -> itree (State +' E)  S) e,
+    interp_asl (t >>= k) e ≈
+       '(e',x) <- interp_asl t e ;; interp_asl (k x) e'.
+Proof.
+  intros.
+  unfold interp_asl.  
+  rewrite interp_bind.
+  unfold MapDefault.interp_map.
+  rewrite interp_state_bind .
+  apply eutt_eq_bind.
+  intros (? & ?).
   reflexivity.
 Qed.
 
