src/ASL/AST.v
@@ -3,10 +3,17 @@ From Coq Require Import Strings.String.
 (* We need to import the Vellvm int32*)
 From Vellvm Require Import Semantics.DynamicValues.
 
+Inductive dec :=
+  | Var (x:string).
+
+Definition decs := list dec.
+
 Inductive expr : Type :=
 | Lit (_ : int32).
 
 Inductive stmt : Type :=
 | Assign (x : string) (e : expr)
-| Seq    (a b : stmt)
 | Skip.
+
+Definition prog := list stmt.
+
