src/Compiler/Compiler.v
@@ -1,46 +1,53 @@
-From Coq    Require Import String BinNat List ZArith.
+From Coq    Require Import Strings.String BinNat List ZArith ListSet.
 From ASL    Require Import AST.
 From Vellvm Require Import Syntax Semantics.
+From ExtLib Require Import Core.RelDec Data.String Data.Map.FMapAList . 
 
 Import ListNotations.
 
 Open Scope list_scope.
 
+
+
+
 (* First we need to extract all the variables initialized inside an ASL program *)
 Section Allocations.
 
-  Fixpoint eqb s1 s2 : bool :=
-   match s1, s2 with
-   | EmptyString, EmptyString => true
-   | String c1 s1', String c2 s2' => Ascii.eqb c1 c2 && eqb s1' s2'
-   | _,_ => false
-   end.
 
-  Fixpoint is_present (s : string) (l : list string) (b : bool) : bool :=
-    match l with
-    | h::tail => is_present s tail (orb b (eqb h s))
-    | [] => b
-    end.
-
-  Fixpoint extract_vars (p : AST.stmt) (l : list string) : list string :=
+(* (*   Fixpoint gen_alloc_instrs (p : AST.stmt) (l : alist (instr_id * instr dtyp) unit) : alist (instr_id * instr dtyp) unit :=
     match p with
     | Skip => l
-    | Seq s1 s2 => extract_vars s2 (extract_vars s1 l)
-    | Assign x e => if (is_present x l false) then l else (x::l) 
+    | Seq s1 s2 => fold_alist alist_add (gen_alloc_instrs s2 nil) (gen_alloc_instrs s1 nil)
+    | Assign x e => alist_add (IId (Name x), (INSTR_Alloca (DTYPE_I 32%N) None None)) tt l 
+    end.
+ *)
+   Fixpoint extract_vars (p : AST.stmt) (l : alist string unit) : alist string unit :=
+    match p with
+    | Skip => l
+    | Seq s1 s2 => fold_alist alist_add (extract_vars s2 nil) (extract_vars s1 nil)
+    | Assign x e => l 
     end.
 
-  Definition gen_alloc_instr (x:string) : instr_id * instr dtyp :=
-    (IId (Name x), (INSTR_Alloca (DTYPE_I 32%N) None None)).
+  Definition gen_alloc_instr (pair : (string * unit)): instr_id * instr dtyp :=
+    (IId (Name (fst pair)), (INSTR_Alloca (DTYPE_I 32%N) None None)).
 
   Definition gen_alloc_code (p : AST.stmt) : code dtyp :=
     let var_list := extract_vars p nil in
       map gen_alloc_instr var_list.
 
+  Fixpoint gen_decs_code (d : AST.decs) : code dtyp :=
+    match d with
+    | Dec x => [gen_alloc_instr (x, tt)]
+    | DecSeq d1 d2 => gen_decs_code d1 ++ gen_decs_code d2
+    end. *)
+
+  
+
 End Allocations.
 
 
 
-(* Given an ASL program, generate the instructions assuming the variables have been previously allocated *)
+(* (* Given an ASL program, generate the instructions assuming the variables have been previously allocated *)
 Fixpoint gen_body_code (p : AST.stmt) : code dtyp :=
   match p with
   | Skip => nil
@@ -50,26 +57,44 @@ Fixpoint gen_body_code (p : AST.stmt) : code dtyp :=
                   end
   end.
 
-(* This function generates a cfg without args, with just one code block labeled as 0 which always return 1 and with code "c" *)
-Definition generate_cfg (c : code dtyp) : cfg dtyp := 
-  {| init := (Anon 0%Z);
-     blks := [{|
-                blk_id    := (Anon 0%Z);
-                blk_phis  := nil;
-                blk_code  := c;
-                blk_term  := TERM_Ret ((DTYPE_I 32%N), (EXP_Integer (1)%Z));
-                blk_comments := None
-              |} ];
-     args := nil |} .
-
-
 (* Convert a program in ASL AST form, into a LLVM AST form *)
-Definition compile (p : AST.stmt) : code dtyp :=
+Definition compile_body (p : AST.stmt) : code dtyp :=
   let alloc_code := gen_alloc_code p in
   let body_code  := gen_body_code  p in
-  body_code.
+  alloc_code ++ body_code.
 
-   
+
+Fixpoint compile_prog (p : AST.prog) : code dtyp :=
+  match p with
+  | Prog d s => gen_decs_code d ++ gen_body_code s
+  end.
+
+
+
+Definition sub  (k : string) (v : unit) (m : alist string unit) :=
+match (alist_find k m) with
+  | Some _ => alist_remove k m
+  | None => m
+end.
+
+Definition alist_sub (m1 m2 : alist string unit) : alist string unit :=
+fold_alist sub m1 m2.
+ *)
+
+Fixpoint gen_body_code (p : AST.stmt) : code dtyp :=
+  match p with
+  | Skip => nil
+  | Assign x v => match v with 
+                  | Lit n => [(IVoid 0%Z, (INSTR_Store false ((DTYPE_I 32%N), (EXP_Integer (Int32.unsigned n))) (DTYPE_Pointer, (EXP_Ident (ID_Local (Name x)))) None))]
+                  end
+  end.
+
+
+Fixpoint compile (p : AST.prog) : code dtyp :=
+  match p with
+  | nil => nil
+  | x :: t => (gen_body_code x) ++ (compile t)
+  end.
 
 
 
